some proofs to help with SCE

lean-sce/LeanSce/Core/Typing.lean
@@ -2,103 +2,40 @@ import LeanSce.Core.Syntax
 
 open Core
 
-/--
-  `HasType E e A` means: under environment type `E`, expression `e` has type `A`.
-
-  Note: the environment is a *type* (not a context list). The `ctx` expression
-  returns the current environment, `box` switches environments, and `mrg`
-  extends the environment.
--/
 inductive HasType : Typ → Exp → Typ → Prop where
-  /-
-    Γ ⊢ ? : Γ
-  -/
   | tquery {Γ : Typ}
     : HasType Γ .query Γ
-  /-
-    Γ ⊢ i : Int
-  -/
   | tint {Γ : Typ} {i : Nat}
     : HasType Γ (.lit i) .int
-  /-
-    Γ ⊢ () : ()
-  -/
   | tunit {Γ : Typ}
     : HasType Γ .unit .top
-  /-
-    Γ ⊢ e₁ : A → B
-    Γ ⊢ e₂ : A
-    ───────────────
-    Γ ⊢ e₁ e₂ : B
-  -/
   | tapp {Γ A B : Typ} {e₁ e₂ : Exp}
     : HasType Γ e₁ (.arr A B)
     → HasType Γ e₂ B
     → HasType Γ (.app e₁ e₂) B
-  /-
-    Γ ⊢ e₁ : Γ₁
-    Γ₁ ⊢ e₂ : A
-    ────────────────
-    Γ ⊢ e₁ ▷ e₂ : A
-  -/
   | tbox {Γ Γ₁ A B : Typ} {e₁ e₂ : Exp}
     : HasType Γ e₁ Γ₁
     → HasType Γ₁ e₂ A
     → HasType Γ (.box e₁ e₂) A
-  /-
-    Γ ⊢ e₁ : A
-    Γ & A ⊢ e₂ : B
-    ────────────────────
-    Γ ⊢ e₁ ,, e₂ : A & B
-  -/
   | tmrg {Γ A B : Typ} {e₁ e₂ : Exp}
     : HasType Γ e₁ A
     → HasType (.and Γ A) e₂ B
     → HasType Γ (.mrg e₁ e₂) (.and A B)
-  /-
-    Γ & A ⊢ e : B
-    ────────────────────
-    Γ ⊢ λA. e : A → B
-  -/
   | tlam {Γ A B : Typ} {e : Exp}
     : HasType (.and Γ A) e B
     → HasType Γ (.lam A e) (.arr A B)
-  /-
-    Γ ⊢ e : A
-    lookup(A, n) = B
-    ─────────────────
-    Γ ⊢ e.n : B
-  -/
   | tproj {Γ A B : Typ} {e : Exp} {n : Nat}
     : HasType Γ e A
     → Lookup A n B
     → HasType Γ (.proj e n) B
-  /-
-    value v
-    () ⊢ v : Γ₁
-    Γ₁ & A ⊢ e : B
-    ─────────────────
-    Γ ⊢ ⟨v, λA. e⟩ : A → B
-  -/
   | tclos {Γ Γ₁ A B : Typ} {v e : Exp} {n : Nat}
     : Value v
     → HasType .top v Γ₁
     → HasType (.and Γ₁ A) e B
     → HasType Γ (.clos v A e) (.arr A B)
-  /-
-    Γ ⊢ e : A
-    ─────────────────────
-    Γ ⊢ {l = e} : {l : A}
-  -/
   | trcd {Γ A : Typ} {l : String} {e : Exp}
     : HasType Γ e A
     → HasType Γ (.lrec l e) (.rcd l A)
-  /-
-    Γ ⊢ e : B
-    rlookup(B, l) = A
-    ───────────────
-    Γ ⊢ e.l : A
-  -/
   | trproj {Γ A B : Typ} {l : String} {e : Exp}
     : HasType Γ e B
     → RLookup B l A
