lean-sce/LeanSce/Core/Theories.lean
@@ -1,0 +1,51 @@
+
+import LeanSce.Core.Syntax
+import LeanSce.Core.Semantics
+import LeanSce.Core.Typing
+
+open Core C_Sem
+
+@[simp]
+theorem value_weaken
+  {E A : Typ} { v : Exp}
+  {htype : HasType E v A} :
+  ∀ {E' : Typ},
+    Value v
+    → HasType E' v A := by
+  induction htype with
+  | tint          => intro _ _; exact .tint
+  | tunit         => intro _ _; exact .tunit
+  | trcd ht ih    => intro _ hv; cases hv; exact .trcd (ih ‹_›)
+  | tlam _        => intro _ hv; cases hv
+  | tquery        => intro _ hv; cases hv
+  | tapp _ _      => intro _ hv; cases hv
+  | tbox _ _      => intro _ hv; cases hv
+  | tproj _ _     => intro _ hv; cases hv
+  | trproj _ _    => intro _ hv; cases hv
+  | tmrg h1 h2 ih1 ih2 =>
+    intro _ hv
+    cases hv with
+    | vmrg hv1 hv2 => exact .tmrg (ih1 hv1) (ih2 hv2)
+  | tclos hv' ht' hb ih1 ih2 =>
+    rename_i Γ₁ Γ₂ A' B' v₀ e₀ n
+    intro E' hv
+    apply HasType.tclos
+    · assumption
+    · assumption
+    · exact (ih1 ∘ fun a => hv') E
+    · assumption
+
+theorem Gpreservation
+  {E A : Typ} {e e' v' : Exp} {hv : Value v'}
+  (hstep : Step v' e e')
+  (htype : HasType E e A)
+  (henv  : HasType .top v' E) :
+  HasType E e' A := by
+  induction hstep with
+  | squery heval =>
+    rename_i v
+    cases htype
+    apply value_weaken; try assumption
+    apply hv
+  | _ =>
+    sorry
